main.v
@@ -1,5 +1,6 @@
 From Prelude Require Import Text.
-From FreeSpec Require Import Exec Console.
-From MiniHTTPServer Require Import Server Exec HTTP.
+From FreeSpec Require Import Core Exec Console.
+From MiniHTTPServer Require Import Server Exec TCP FileSystem HTTP URI.
+From Comparse Require Import Combinators.
 
 Exec http_server.
